HOL/SepLogic/Connectivity_Impl.thy
@@ -10,14 +10,13 @@ fun connected_rel_imp :: "nat \<Rightarrow> (nat \<times> nat) list \<Rightarrow
     p \<leftarrow> connected_rel_imp n es k;
     p' \<leftarrow> uf_union p (fst (es ! k)) (snd (es ! k));
     return p' }"
-declare connected_rel_imp.simps [sep_proc_defs]
+declare connected_rel_imp.simps [sep_proc]
 
 lemma connected_rel_imp_to_fun [hoare_triple]:
   "<\<up>(is_valid_graph n (set es)) * \<up>(k \<le> length es)>
    connected_rel_imp n es k
    <is_uf n (connected_rel_ind n es k)>"
 @proof @induct k @qed
-declare connected_rel_imp.simps [sep_proc_defs del]
 
 lemma connected_rel_imp_correct [hoare_triple]:
   "<\<up>(is_valid_graph n (set es))>
