HOL/SepLogic/Union_Find_Impl.thy
@@ -9,7 +9,7 @@ definition is_uf :: "nat \<Rightarrow> (nat\<times>nat) set \<Rightarrow> uf \<R
         \<up>(ufa_invar l \<and> ufa_\<alpha> l = R \<and> length l = n \<and> length szl = n))"
 setup {* add_rewrite_ent_rule @{thm is_uf_def} *}
 
-definition uf_init :: "nat \<Rightarrow> uf Heap" where [sep_proc_defs]:
+definition uf_init :: "nat \<Rightarrow> uf Heap" where [sep_proc]:
   "uf_init n = do {
      l \<leftarrow> Array.of_list [0..<n];
      szl \<leftarrow> Array.new n (1::nat);
@@ -18,14 +18,13 @@ definition uf_init :: "nat \<Rightarrow> uf Heap" where [sep_proc_defs]:
 
 lemma uf_init_rule [hoare_triple]:
   "<emp> uf_init n <is_uf n (uf_init_rel n)>" by auto2
-declare uf_init_def [sep_proc_defs del]
   
 partial_function (heap) uf_rep_of :: "nat array \<Rightarrow> nat \<Rightarrow> nat Heap" where
   "uf_rep_of p i = do {
      n \<leftarrow> Array.nth p i;
      if n = i then return i else uf_rep_of p n
    }"
-declare uf_rep_of.simps [sep_proc_defs]
+declare uf_rep_of.simps [sep_proc]
   
 lemma uf_rep_of_rule [hoare_triple]:
   "ufa_invar l \<Longrightarrow> i < length l \<Longrightarrow>
@@ -33,7 +32,6 @@ lemma uf_rep_of_rule [hoare_triple]:
    uf_rep_of p i
    <\<lambda>r. p \<mapsto>\<^sub>a l * \<up>(r = rep_of l i)>"
 @proof @prop_induct "ufa_invar l \<and> i < length l" @qed
-declare uf_rep_of.simps [sep_proc_defs del]
 
 partial_function (heap) uf_compress :: "nat \<Rightarrow> nat \<Rightarrow> nat array \<Rightarrow> unit Heap" where
   "uf_compress i ci p = (
@@ -44,7 +42,7 @@ partial_function (heap) uf_compress :: "nat \<Rightarrow> nat \<Rightarrow> nat 
       Array.upd i ci p;
       return ()
     })"
-declare uf_compress.simps [sep_proc_defs]
+declare uf_compress.simps [sep_proc]
 
 lemma uf_compress_rule [hoare_triple]:
   "ufa_invar l \<Longrightarrow> i < length l \<Longrightarrow>
@@ -52,9 +50,8 @@ lemma uf_compress_rule [hoare_triple]:
    uf_compress i (rep_of l i) p
    <\<lambda>_. \<exists>\<^sub>Al'. p \<mapsto>\<^sub>a l' * \<up>(ufa_invar l' \<and> length l' = length l \<and> (\<forall>i<length l. rep_of l' i = rep_of l i))>"
 @proof @prop_induct "ufa_invar l \<and> i < length l" @qed
-declare uf_compress.simps [sep_proc_defs del]
 
-definition uf_rep_of_c :: "nat array \<Rightarrow> nat \<Rightarrow> nat Heap" where [sep_proc_defs]:
+definition uf_rep_of_c :: "nat array \<Rightarrow> nat \<Rightarrow> nat Heap" where [sep_proc]:
   "uf_rep_of_c p i = do {
     ci \<leftarrow> uf_rep_of p i;
     uf_compress i ci p;
@@ -68,9 +65,8 @@ lemma uf_rep_of_c_rule [hoare_triple]:
    <\<lambda>r. \<exists>\<^sub>Al'. p \<mapsto>\<^sub>a l' * \<up>(r = rep_of l i \<and> ufa_invar l' \<and> length l' = length l \<and>
                           (\<forall>i<length l. rep_of l' i = rep_of l i))>"
   by auto2
-declare uf_rep_of_c_def [sep_proc_defs del]
 
-definition uf_cmp :: "uf \<Rightarrow> nat \<Rightarrow> nat \<Rightarrow> bool Heap" where [sep_proc_defs]:
+definition uf_cmp :: "uf \<Rightarrow> nat \<Rightarrow> nat \<Rightarrow> bool Heap" where [sep_proc]:
   "uf_cmp u i j \<equiv> do {
     n \<leftarrow> Array.len (snd u);
     if (i\<ge>n \<or> j\<ge>n) then return False
@@ -85,9 +81,8 @@ lemma uf_cmp_rule [hoare_triple]:
   "<is_uf n R u>
    uf_cmp u i j
    <\<lambda>r. is_uf n R u * \<up>(r \<longleftrightarrow> (i,j)\<in>R)>" by auto2
-declare uf_cmp_def [sep_proc_defs del]
 
-definition uf_union :: "uf \<Rightarrow> nat \<Rightarrow> nat \<Rightarrow> uf Heap" where [sep_proc_defs]:
+definition uf_union :: "uf \<Rightarrow> nat \<Rightarrow> nat \<Rightarrow> uf Heap" where [sep_proc]:
   "uf_union u i j \<equiv> do {
     ci \<leftarrow> uf_rep_of (snd u) i;
     cj \<leftarrow> uf_rep_of (snd u) j;
@@ -112,6 +107,5 @@ lemma uf_union_rule [hoare_triple]:
    <is_uf n R u>
    uf_union u i j
    <is_uf n (per_union R i j)>" by auto2
-declare uf_union_def [sep_proc_defs del]
 
 end
